refactored bytewise

refinedVST/typing/bytes.v
@@ -2,6 +2,7 @@ Set Warnings "-notation-overridden,-custom-entry-overridden,-hiding-delimiting-k
 From VST.typing Require Export type.
 From VST.typing Require Import programs int own.
 Set Warnings "notation-overridden,custom-entry-overridden,hiding-delimiting-key".
+From VST.floyd Require Import encode_reptype.
 From VST.typing Require Import type_options.
 
 (* NOTE: we might want to have a type [bytes : list mbyte → type] one day,
@@ -9,137 +10,10 @@ and the [bytewise] abstraction could be encoded on top of it. *)
 
 Section bytewise.
   Context `{!typeG OK_ty Σ} {cs : compspecs}.
-
-  Opaque field_type.
+  Implicit Types P : memval → Prop.
 
   (* Because ty_own_val is at the reptype level, for now this is defined only for bytewise representations
      of reptypes, rather than arbitrary byte arrays that happen to have the right layout. *)
-
-  Definition struct_encode_aux (m m0: members) (sz: Z)
-       (P: hlist.hlist (type_induction.tmap (fun it => reptype (field_type (name_member it) m0) -> list memval) m))
-       (v: compact_prod (map (fun it => reptype (field_type (name_member it) m0)) m)) : list memval.
-  Proof.
-    destruct m as [| a0 m]; [exact [] |].
-    revert a0 v P; induction m as [| a0 m]; intros ? v P.
-    + simpl in v, P.
-      inversion P; subst.
-      exact (X v ++ Zrepeat Undef (field_offset_next cenv_cs (name_member a0) m0 sz - (field_offset cenv_cs (name_member a0) m0 + sizeof (field_type (name_member a0) m0)))).
-    + simpl in v, P.
-      inversion P; subst.
-      exact (X (fst v) ++ Zrepeat Undef (field_offset_next cenv_cs (name_member a1) m0 sz - (field_offset cenv_cs (name_member a1) m0 + sizeof (field_type (name_member a1) m0))) ++
-        IHm a0 (snd v) X0).
-  Defined.
-
-  Definition struct_encode (m: members) {A : member → Type} (P : ∀ it, A it → list memval) (v: compact_prod (map A m)) : list memval.
-  Proof.
-    destruct m as [| a m]; [exact [] | ].
-    revert a v; induction m as [| b m]; intros ? v.
-    + simpl in v.
-      exact (P _ v).
-    + simpl in v.
-      exact (P _ (fst v) ++ IHm _ (snd v)).
-  Defined.
-
-  Lemma struct_encode_aux_spec: forall m m0 sz v P,
-    struct_encode_aux m m0 sz
-      (type_induction.hmap (fun it => reptype (field_type (name_member it) m0) -> list memval) P m) v =
-    struct_encode m (fun it v => P it v ++
-      Zrepeat Undef (field_offset_next cenv_cs (name_member it) m0 sz - (field_offset cenv_cs (name_member it) m0 + sizeof (field_type (name_member it) m0)))) v.
-  Proof.
-    intros.
-    destruct m as [| a0 m]; [reflexivity |].
-    revert a0 v; induction m as [| a0 m]; intros.
-    + reflexivity.
-    + change (struct_encode_aux (a1 :: a0 :: m) m0 sz
-     (type_induction.hmap (fun it : member => reptype (field_type (name_member it) m0) -> list memval)
-        P (a1 :: a0 :: m)) v) with
-     (P a1 (fst v) ++ Zrepeat Undef (field_offset_next cenv_cs (name_member a1) m0 sz - (field_offset cenv_cs (name_member a1) m0 + sizeof (field_type (name_member a1) m0))) ++
-      struct_encode_aux (a0 :: m) m0 sz
-        (type_induction.hmap (fun it : member => reptype (field_type (name_member it) m0) -> list memval)
-        P (a0 :: m)) (snd v)).
-      rewrite IHm app_assoc //.
-  Qed.
-
-  Definition union_encode_aux (m m0: members) (sz: Z)
-      (P: hlist.hlist (type_induction.tmap (fun it => reptype (field_type (name_member it) m0) -> list memval) m))
-      (v: compact_sum (map (fun it => reptype (field_type (name_member it) m0)) m)) : list memval.
-  Proof.
-    destruct m as [| a0 m]; [exact [] |].
-    revert a0 v P; induction m as [| a0 m]; intros ? v P.
-    + simpl in v, P.
-      inversion P; subst.
-      exact (X v ++ Zrepeat Undef (sz - sizeof (field_type (name_member a0) m0))).
-    + simpl in v, P.
-      inversion P; subst.
-      destruct v as [v | v].
-      - exact (X v ++ Zrepeat Undef (sz - sizeof (field_type (name_member a1) m0))).
-      - exact (IHm a0 v X0).
-  Defined.
-
-  Definition union_encode (m: members) {A : member → Type} (P : ∀ it, A it → list memval) (v: compact_sum (map A m)) : list memval.
-  Proof.
-    destruct m as [| a m]; [exact [] | ].
-    revert a v; induction m as [| b m]; intros ? v.
-    + simpl in v.
-      exact (P _ v).
-    + simpl in v.
-      destruct v as [v | v].
-      - exact (P _ v).
-      - exact (IHm _ v).
-  Defined.
-
-  Lemma union_encode_aux_spec: forall m m0 sz v P,
-    union_encode_aux m m0 sz
-      (type_induction.hmap (fun it => reptype (field_type (name_member it) m0) -> list memval) P m) v =
-    union_encode m (fun it v => P it v ++
-      Zrepeat Undef (sz - sizeof (field_type (name_member it) m0))) v.
-  Proof.
-    intros.
-    destruct m as [| a0 m]; [reflexivity |].
-    revert a0 v; induction m as [| a0 m]; intros.
-    + reflexivity.
-    + destruct v as [v | v].
-      - reflexivity.
-      - match goal with
-        | _ => apply IHm
-        | _ => simpl; f_equal; apply IHm
-        end.
-  Qed.
-
-  Definition encode_reptype: forall t, reptype t -> list memval :=
-    type_induction.type_func (fun t => reptype t -> list memval)
-      (fun t v => match access_mode t with By_value ch => encode_val ch (repinject t v) | _ => Zrepeat Undef (sizeof t) end)
-      (fun t n a P v => foldr (λ v m, P v ++ m) [] (unfold_reptype v))
-      (fun id a P v => struct_encode_aux (co_members (get_co id)) (co_members (get_co id)) (co_sizeof (get_co id)) P (unfold_reptype v))
-      (fun id a P v => union_encode_aux (co_members (get_co id)) (co_members (get_co id)) (co_sizeof (get_co id)) P (unfold_reptype v)).
-
-  Lemma encode_reptype_eq: forall t v,
-    encode_reptype t v =
-    match t return REPTYPE t -> list memval with
-    | Tvoid
-    | Tfunction _ _ _ => fun _ => [Undef]
-    | Tint _ _ _
-    | Tfloat _ _
-    | Tlong _ _
-    | Tpointer _ _ => fun v => match access_mode t with By_value ch => encode_val ch v | _ => Zrepeat Undef (sizeof t) end
-    | Tarray t0 n a => fun v => foldr (λ v m, encode_reptype t0 v ++ m) [] v
-    | Tstruct id a => struct_encode (co_members (get_co id)) (fun it v => encode_reptype (field_type (name_member it) (co_members (get_co id))) v ++
-        Zrepeat Undef (field_offset_next cenv_cs (name_member it) (co_members (get_co id)) (co_sizeof (get_co id)) -
-          (field_offset cenv_cs (name_member it) (co_members (get_co id)) + sizeof (field_type (name_member it) (co_members (get_co id))))))
-    | Tunion id a => union_encode (co_members (get_co id)) (fun it v => encode_reptype (field_type (name_member it) (co_members (get_co id))) v ++
-        Zrepeat Undef ((co_sizeof (get_co id)) - sizeof (field_type (name_member it) (co_members (get_co id)))))
-    end (unfold_reptype v).
-  Proof.
-    intros.
-    unfold encode_reptype at 1.
-    rewrite type_induction.type_func_eq.
-    destruct t; auto.
-    + rewrite <- struct_encode_aux_spec; reflexivity.
-    + rewrite <- union_encode_aux_spec; reflexivity.
-  Qed.
-
-  Implicit Types P : memval → Prop.
-
   Program Definition bytewise (P : memval → Prop) (cty : Ctypes.type) : type := {|
     ty_has_op_type ot mt := ot = cty;
     ty_own β l :=
